Make ToyClient resolve, verify, compile, and run (#34)
* Make ToyClient resolve, verify, compile, and run

Update Makefile to include all the files needed.
Update Makefile to split build and verify targets (which makes it easy to rebuild without verifying everything).
Rewrite Main to only use the RSA keyring (not a multi-keyring with both RSA and AES).
Reintroduc `EC_PUBLIC_KEY_FIELD` constant in Materials.dfy.
Mark some recursive routines in StandardLibrary with `{:opaque}`, which will improve verifier performance.

Note, although I did fix up most of the formatting, I did not change all variables names according to our conventions.

We still need to compare the specs and code to the English specification. This PR is not intended to address the various Issues we have recorded as TODOs.

`make` comes out clean.

src/SDK/Keyring/RSAKeyring.dfy
@@ -1,113 +1,127 @@
-include "../MessageHeader/Definitions.dfy"
 include "../../StandardLibrary/StandardLibrary.dfy"
 include "../../StandardLibrary/UInt.dfy"
+include "../Materials.dfy"
+include "Defs.dfy"
 include "../AlgorithmSuite.dfy"
-include "./Defs.dfy"
-include "../../Crypto/Cipher.dfy"
 include "../../Crypto/GenBytes.dfy"
 include "../../Crypto/RSAEncryption.dfy"
-include "../Materials.dfy"
 
 module RSAKeyringDef {
-    import opened KeyringDefs
-    import opened StandardLibrary
-    import opened UInt = StandardLibrary.UInt
-    import opened Cipher
-    import GenBytes = RNG
-    import AlgorithmSuite
-    import RSA = RSAEncryption
-    import opened SDKDefs
+  import opened StandardLibrary
+  import opened UInt = StandardLibrary.UInt
+  import KeyringDefs
+  import AlgorithmSuite
+  import RSA = RSAEncryption
+  import Materials
+  import RNG
 
-    class RSAKeyring extends Keyring {
-        const key_namespace : seq<uint8>
-        const key_name : seq<uint8>
-        const rsa_params : (RSA.RSAPaddingMode, RSA.RSABitLength)
-        const enc_key : Option<seq<uint8>>
-        const dec_key : Option<seq<uint8>>
+  class RSAKeyring extends KeyringDefs.Keyring {
+    const keyNamespace: seq<uint8>
+    const keyName: seq<uint8>
+    const paddingMode: RSA.RSAPaddingMode
+    const bitLength: RSA.RSABitLength
+    const encryptionKey: Option<seq<uint8>>
+    const decryptionKey: Option<seq<uint8>>
 
-        predicate Valid() reads this {
-            Repr == {this} &&
-            (enc_key.Some? ==> RSA.RSA.RSAWfEK(rsa_params.1, rsa_params.0, enc_key.get)) &&
-            (dec_key.Some? ==> RSA.RSA.RSAWfDK(rsa_params.1, rsa_params.0, dec_key.get)) &&
-            (enc_key.Some? || dec_key.Some?)
-        }
-
-        constructor(namespace : seq<uint8>, name : seq<uint8>, padding : RSA.RSAPaddingMode, bits : RSA.RSABitLength, ek: Option<seq<uint8>>, dk: Option<seq<uint8>>)
-            requires ek.Some? ==> RSA.RSA.RSAWfEK(bits, padding, ek.get)
-            requires dk.Some? ==> RSA.RSA.RSAWfDK(bits, padding, dk.get)
-            requires (ek.Some? || dk.Some?)
-            ensures key_namespace == namespace
-            ensures key_name == name
-            ensures rsa_params == (padding, bits)
-            ensures enc_key == ek
-            ensures dec_key == dk
-            ensures Valid()
-        {
-            key_namespace := namespace;
-            key_name := name;
-            rsa_params := (padding, bits);
-            enc_key := ek;
-            dec_key := dk;
-            Repr := {this};
-        }
-
-        method OnEncrypt(x : EncMaterials) returns (res : Result<EncMaterials>)
-            requires WFEncMaterials(x)
-            requires Valid() ensures Valid()
-            ensures res.Ok? ==> WFEncMaterials(res.get)
-            ensures res.Ok? ==> res.get.alg_id == x.alg_id
-            ensures enc_key.None? ==> res.Err?
-        {
-            if enc_key.None? {
-                res := Err("Encryption key undefined");
-            }
-            else {
-                var data_key := x.data_key;
-                var alg_id := x.alg_id;
-                if data_key.None? {
-                    var k := RNG.GenBytes(AlgorithmSuite.input_key_length(alg_id) as uint16);
-                    data_key := Some(k);
-                }
-                var aad := FlattenSortEncCtx(x.enc_ctx);
-                var edk_ctxt := RSA.RSA.RSAEncrypt(rsa_params.1, rsa_params.0, enc_key.get, data_key.get);
-                if edk_ctxt.None? { return Err("Error on encrypt!"); }
-                var provider_id := key_namespace;
-                var provider_info := key_name;
-                return Ok(EncMat((alg_id), [EDK(provider_id, provider_info, edk_ctxt.get)] + x.edks, x.enc_ctx, data_key, None));
-
-            }
-
-        }
-
-
-        method OnDecrypt(x : DecMaterials, edks : seq<EDK>) returns (res : Result<DecMaterials>)
-            requires Valid()
-            requires WFDecMaterials(x)
-            ensures Valid()
-            ensures res.Ok? ==> WFDecMaterials(res.get)
-            ensures res.Ok? ==> res.get.alg_id == x.alg_id
-            ensures dec_key.None? ==> res.Err?
-        {
-            if dec_key.None? { return Err(("Decryption key undefined"));}
-            if |edks| == 0 { return Err(("Ran out of edks")); }
-            if edks[0].provider_id != key_namespace { var x := OnDecrypt(x, edks[1..]); return x;}
-            if edks[0].provider_info != key_name { var x := OnDecrypt(x, edks[1..]); return x;}
-            var octxt := RSA.RSA.RSADecrypt(rsa_params.1, rsa_params.0, dec_key.get, edks[0].ciphertext);
-            match octxt {
-                    case None => {var x := OnDecrypt(x, edks[1..]); return x;}
-                    case Some(k) => {
-                            if |k| == AlgorithmSuite.input_key_length(x.alg_id) { // check for correct key length
-                                return Ok(DecMat(x.alg_id, x.enc_ctx, Some(k), None));
-                            }
-                            else {
-                                return Err(("Bad key length!"));
-                            }
-                    }
-
-            }
-        }
-
-
+    predicate Valid()
+      reads this
+    {
+      Repr == {this} &&
+      (encryptionKey.Some? ==> RSA.RSA.RSAWfEK(bitLength, paddingMode, encryptionKey.get)) &&
+      (decryptionKey.Some? ==> RSA.RSA.RSAWfDK(bitLength, paddingMode, decryptionKey.get)) &&
+      (encryptionKey.Some? || decryptionKey.Some?)
     }
 
+    constructor(namespace: seq<uint8>, name: seq<uint8>, padding: RSA.RSAPaddingMode, bits: RSA.RSABitLength, ek: Option<seq<uint8>>, dk: Option<seq<uint8>>)
+      requires ek.Some? ==> RSA.RSA.RSAWfEK(bits, padding, ek.get)
+      requires dk.Some? ==> RSA.RSA.RSAWfDK(bits, padding, dk.get)
+      requires ek.Some? || dk.Some?
+      ensures keyNamespace == namespace
+      ensures keyName == name
+      ensures paddingMode == padding && bitLength == bits
+      ensures encryptionKey == ek
+      ensures decryptionKey == dk
+      ensures Valid()
+    {
+      keyNamespace := namespace;
+      keyName := name;
+      paddingMode, bitLength := padding, bits;
+      encryptionKey := ek;
+      decryptionKey := dk;
+      Repr := {this};
+    }
+
+    method OnEncrypt(encMat: Materials.EncryptionMaterials) returns (res: Result<Materials.EncryptionMaterials>)
+      requires Valid()
+      requires encMat.Valid()
+      modifies encMat`plaintextDataKey, encMat`encryptedDataKeys
+      ensures Valid()
+      ensures res.Success? ==> res.value.Valid() && res.value == encMat
+      ensures res.Success? && old(encMat.plaintextDataKey.Some?) ==> res.value.plaintextDataKey == old(encMat.plaintextDataKey)
+      ensures res.Failure? ==> unchanged(encMat)
+    {
+      if encryptionKey.None? {
+        res := Failure("Encryption key undefined");
+      } else {
+        var dataKey := encMat.plaintextDataKey;
+        var algorithmID := encMat.algorithmSuiteID;
+        if dataKey.None? {
+          var k := RNG.GenBytes(algorithmID.KeyLength() as uint16);
+          dataKey := Some(k);
+        }
+        var aad := Materials.FlattenSortEncCtx(encMat.encryptionContext);
+        var edkCiphertext := RSA.RSA.RSAEncrypt(bitLength, paddingMode, encryptionKey.get, dataKey.get);
+        if edkCiphertext.None? {
+          return Failure("Error on encrypt!");
+        }
+        var edk := Materials.EncryptedDataKey(ByteSeqToString(keyNamespace), keyName, edkCiphertext.get);
+        encMat.encryptedDataKeys := [edk] + encMat.encryptedDataKeys;
+        encMat.plaintextDataKey := dataKey;
+        return Success(encMat);
+      }
+    }
+
+    method OnDecrypt(decMat: Materials.DecryptionMaterials, edks: seq<Materials.EncryptedDataKey>) returns (res: Result<Materials.DecryptionMaterials>)
+      requires Valid()
+      requires decMat.Valid()
+      modifies decMat`plaintextDataKey
+      ensures Valid()
+      ensures decMat.Valid()
+      ensures |edks| == 0 ==> res.Success? && unchanged(decMat)
+      ensures old(decMat.plaintextDataKey.Some?) ==> res.Success? && unchanged(decMat)
+      ensures res.Success? ==> res.value == decMat
+      ensures res.Failure? ==> unchanged(decMat)
+    {
+      if decMat.plaintextDataKey.Some? || |edks| == 0 {
+        return Success(decMat);
+      } else if decryptionKey.None? {
+        return Failure("Decryption key undefined");
+      }
+      var i := 0;
+      while i < |edks|
+        invariant  0 <= i <= |edks|
+      {
+        var edk := edks[i];
+        if edk.providerID != ByteSeqToString(keyNamespace) {
+          // continue with the next EDK
+        } else if edk.providerInfo != keyName {
+          // continue with the next EDK
+        } else {
+          var octxt := RSA.RSA.RSADecrypt(bitLength, paddingMode, decryptionKey.get, edks[0].ciphertext);
+          match octxt
+          case None =>
+            // continue with the next EDK
+          case Some(k) =>
+            if |k| == decMat.algorithmSuiteID.KeyLength() { // check for correct key length
+              decMat.plaintextDataKey := Some(k);
+              return Success(decMat);
+            } else {
+              return Failure(("Bad key length!"));
+            }
+        }
+        i := i + 1;
+      }
+      return Success(decMat);
+    }
+  }
 }
