src/Main.dfy
@@ -1,59 +1,91 @@
 include "SDK/ToyClient.dfy"
-include "SDK/Keyring/AESKeyring.dfy"
+//include "SDK/Keyring/AESKeyring.dfy"
 include "SDK/Keyring/RSAKeyring.dfy"
-include "SDK/Keyring/MultiKeyring.dfy"
-include "SDK/Keyring/Defs.dfy"
+//include "SDK/Keyring/MultiKeyring.dfy"
+//include "SDK/Keyring/Defs.dfy"
 include "SDK/Materials.dfy"
-include "Crypto/AESEncryption.dfy"
-include "Crypto/RSAEncryption.dfy"
-include "Crypto/Signature.dfy"
-include "Crypto/Cipher.dfy"
-include "StandardLibrary/StandardLibrary.dfy"
+//include "Crypto/AESEncryption.dfy"
+//include "Crypto/RSAEncryption.dfy"
+//include "Crypto/Signature.dfy"
+//include "Crypto/Cipher.dfy"
+//include "StandardLibrary/StandardLibrary.dfy"
 include "SDK/CMM/DefaultCMM.dfy"
 
 module Main {
-    import opened ToyClientDef
-    import AES = AESEncryption
-    import RSA = RSAEncryption
-    import opened Cipher
-    import opened AESKeyringDef
-    import K = KeyringDefs
-    import opened RSAKeyringDef
-    import opened StandardLibrary
-    import opened MultiKeyringDef
-    import opened SDKDefs
-    import opened DefaultCMMDef
-    import S = Signature
+  import opened StandardLibrary
+  import opened UInt = StandardLibrary.UInt
+  import DefaultCMMDef
+  import Client = ToyClientDef
+  import RSA = RSAEncryption
+  import RSAKeyringDef
+  import Materials
+  //import AES = AESEncryption
+  //import opened Cipher
+  //import opened AESKeyringDef
+  //import K = KeyringDefs
+  //import opened MultiKeyringDef
+  //import opened SDKDefs
+  //import opened DefaultCMMDef
+  //import S = Signature
 
-    method RunToyClient() {
-        var ek, dk := RSA.RSA.RSAKeygen(2048, RSA.PKCS1);
-        var rsa_kr := new RSAKeyring(byteseq_of_string("namespace"), byteseq_of_string("name"), RSA.PKCS1, 2048, Some(ek), Some(dk));
-        var k2 := AES.AES.AESKeygen(AES_GCM_256);
-        var aes_kr := new AESKeyring(byteseq_of_string("namespace"), byteseq_of_string("name2"), k2, AES_GCM_256);
-        var kr_children := new K.Keyring[1](_ => rsa_kr);
-        var kr := new MultiKeyring(aes_kr, kr_children);
-        var cmm := new DefaultCMM.OfKeyring(kr);
-        var client := new ToyClient.OfCMM(cmm);
+  /*
+  method RunToyClient() {
+    var ek, dk := RSA.RSA.RSAKeygen(2048, RSA.PKCS1);
+    var rsa_kr := new RSAKeyring(byteseq_of_string("namespace"), byteseq_of_string("name"), RSA.PKCS1, 2048, Some(ek), Some(dk));
+    var k2 := AES.AES.AESKeygen(AES_GCM_256);
+    var aes_kr := new AESKeyring(byteseq_of_string("namespace"), byteseq_of_string("name2"), k2, AES_GCM_256);
+    var kr_children := new K.Keyring[1](_ => rsa_kr);
+    var kr := new MultiKeyring(aes_kr, kr_children);
+    var cmm := new DefaultCMM.OfKeyring(kr);
+    var client := new ToyClient.OfCMM(cmm);
 
-        var msg := byteseq_of_string("hello");
-        print "Message: ", msg, "\n";
-        var e := client.Enc(byteseq_of_string("hello"), enc_ctx_of_strings([("keyA", "valA")]));
-            // datatype Encryption = Encryption(ec : EncCtx, edks : seq<EDK>, ciphertext : seq<uint8>)
-        if e.Err? {
-            print "Bad encryption :( ", e.err, "\n";
-            return;
-        }
-        var d := client.Dec(e.get);
-        if d.Err? {
-            print "bad decryption: ", d.err, "\n";
-            return;
-        }
-        print "Produced ", |e.get.edks|, " EDKs \n";
-        print "Decrypted to: ", d.get, "\n";
-        print "AAD: ", string_of_byteseq(FlattenSortEncCtx(e.get.ec)), "\n";
+    var msg := byteseq_of_string("hello");
+    print "Message: ", msg, "\n";
+    var e := client.Enc(byteseq_of_string("hello"), enc_ctx_of_strings([("keyA", "valA")]));
+    // datatype Encryption = Encryption(ec : EncCtx, edks : seq<EDK>, ciphertext : seq<uint8>)
+    if e.Err? {
+      print "Bad encryption :( ", e.err, "\n";
+      return;
     }
-
-    method Main() {
-        RunToyClient();
+    var d := client.Dec(e.get);
+    if d.Err? {
+      print "bad decryption: ", d.err, "\n";
+      return;
     }
+    print "Produced ", |e.get.edks|, " EDKs \n";
+    print "Decrypted to: ", d.get, "\n";
+    print "AAD: ", string_of_byteseq(FlattenSortEncCtx(e.get.ec)), "\n";
+  }
+  */
+
+  method EncryptDecryptTest(client: Client.Client)
+    requires client.Valid()
+  {
+    var msg := StringToByteSeq("hello");
+    print "Message: ", msg, "\n";
+    var e := client.Encrypt(msg, Materials.enc_ctx_of_strings([("keyA", "valA")]));
+    if e.Failure? {
+      print "Bad encryption :( ", e.error, "\n";
+      return;
+    }
+    var d := client.Decrypt(e.value);
+    if d.Failure? {
+      print "bad decryption: ", d.error, "\n";
+      return;
+    }
+    print "Produced ", |e.value.edks|, " EDKs \n";
+    print "Decrypted to: ", d.value, "\n";
+    print "AAD: ", ByteSeqToString(Materials.FlattenSortEncCtx(e.value.ec)), "\n";
+  }
+
+  method Main() {
+    var namespace := StringToByteSeq("namespace");
+    var name := StringToByteSeq("MyKeyring");
+    var ek, dk := RSA.RSA.RSAKeygen(2048, RSA.PKCS1);
+    var keyring := new RSAKeyringDef.RSAKeyring(namespace, name, RSA.RSAPaddingMode.PKCS1, 2048, Some(ek), Some(dk));
+    var cmm := new DefaultCMMDef.DefaultCMM.OfKeyring(keyring);
+    var client := new Client.Client.OfCMM(cmm);
+
+    EncryptDecryptTest(client);
+  }
 }
